LoL/MProp/HoareTriples.lean
@@ -9,10 +9,3 @@ variable [MProp m l]
 
 def triple (pre : m PProp) (c : m α) (post : α -> m PProp) : Prop :=
   MProp.μ pre ≤ liftM (n := Cont l) c (MProp.μ (m := m) ∘ post)
-
-def spec (pre : m PProp) (post : α -> m PProp) : Cont l α :=
-  fun post => MProp.μ pre
-
-lemma tripe_refine (pre : m PProp) (c : m α) (post : α -> m PProp) :
-  triple pre c post →
-  liftM (n := Cont l) c ≤
