LoL/MonadAlgebras/EffectObservations.lean
@@ -23,26 +23,10 @@ class MonadAlgebraOrdered [Monad m] (x : outParam (Type u)) [Preorder x] extends
   bind_le : ∀ {α : Type u} (y : m α) (f f' : α -> x),
     (∀ a, f a ≤ f' a) → morphism (f <$> y) ≤ morphism (f' <$> y)
 
-@[simp]
-def Cont.monotone {t : Type v} {α : Type u} [Preorder t] (wp : Cont t α) :=
-  ∀ (f f' : α -> t), (∀ a, f a ≤ f' a) → wp f ≤ wp f'
-
 lemma Cont.monotone_lift {t : Type u} [Monad m] [LawfulMonad m] [Preorder t] [MonadAlgebraOrdered m t] :
   ∀ {α : Type u} (x : m α), MonadAlgebra.lift x |>.monotone := by
   unfold Cont.monotone; intros; unfold MonadAlgebra.lift
   solve_by_elim [MonadAlgebraOrdered.bind_le]
-
-structure W (t : Type v) [Preorder t] (α : Type u) where
-  wp : Cont t α
-  wp_montone : wp.monotone
-
-@[ext]
-lemma W_ext (t : Type v) (α : Type u) [Preorder t] (w w' : W t α) :
-  w.wp = w'.wp → w = w' := by intros; cases w; cases w'; simp_all
-
-instance (t : Type v) [Preorder t] : Monad (W t) where
-  pure x := ⟨fun f => f x, by solve_by_elim⟩
-  bind x f := ⟨fun g => x.wp (fun a => (f a).wp g), by simp; intros; solve_by_elim [W.wp_montone]⟩
 
 instance (t : Type u) [MonadOrder m] [LawfulMonad m] [Preorder t] [MonadAlgebraOrdered m t] : LawfulMonadLift m (W t) where
   monadLift := fun x => ⟨MonadAlgebra.lift x, Cont.monotone_lift m x⟩
