LoL/MonadAlgebras/Functors.lean
@@ -3,7 +3,7 @@ import LoL.MonadAlgebras.EffectObservations
 
 universe u v w
 
-class TransformerAlgebra (t : (Type u -> Type u) -> (Type u -> Type u)) (m : outParam (Type u -> Type u))
+class TransformerAlgebra (t : (Type u -> Type u) -> (Type u -> Type v)) (m : outParam (Type u -> Type u))
   [Monad m] [inst: MonadTransformer t] where
   hasmorphism {x : Type u} [MonadAlgebra m x] :
-    @MonadAlgebra.{u, u} (t m) inst.isMonad (m x)
+    @MonadAlgebra (t m) inst.isMonad (m x)
