LoL/Tactic.lean
@@ -8,12 +8,13 @@ open Tactic Lean.Meta
 
 
 elab "simp_lift" m:ident : tactic => do
+  let ns <- getCurrNamespace
   let MProp.μ := mkIdent `MProp.μ
   let MProp.μ_lift := mkIdent `MProp.μ_lift
-  let MProp.μ_pure := mkIdent `MProp.μ_pure
+  let MProp.μ_pure := mkIdent <| ns ++ `MProp.μ_pure
   let lift_bind := mkIdent `lift_bind
   let monadMap_if := mkIdent `monadMap_if
-  let cmd <- `(#gen_spec MProp.μ_pure for $MProp.μ (m := $m) ∘ pure)
+  let cmd <- `(#gen_spec $MProp.μ_pure for $MProp.μ (m := $m) ∘ pure)
   liftCommandElabM (Lean.Elab.Command.elabCommand cmd)
   Lean.Elab.Tactic.evalTactic $ <- `(tactic| (
     unfold Function.comp; dsimp
