README.md
@@ -1,1 +1,24 @@
 # LoL
+
+## Interface:
+
+### Total functions
+
+```lean4
+def foo : m a := ...
+
+lemma foo_spec (P : m Prop) (Q : a -> m Prop) : { P } foo { x, Q x } := ...
+```
+
+### Partial functions (Don't know if it will work)
+
+assume `foo` has a `while`-loop or non-structural recursion
+
+first you prove the following total Hoare-logic
+
+```lean4
+
+lemma foo_spec (P : m Prop) (Q : a -> m Prop) : { P } foo { x, Q x } := ...
+```
+This means `foo` terminates, providing `P`. This should give you a total function `foo : P -> m a`. We can run it in Lean by `foo sorryAx`.
+
